theories/Subst/UVarMap.v
@@ -1,0 +1,285 @@
+Require Import Coq.PArith.BinPos.
+Require Import Coq.FSets.FMapPositive.
+Require Import Coq.FSets.FMapInterface.
+Require Import MirrorCore.ExprI.
+
+Set Implicit Arguments.
+Set Strict Implicit.
+
+Let uvar : Type := nat.
+
+Module UVar_ord <: OrderedType.OrderedType with Definition t := uvar
+                                           with Definition eq := @eq uvar.
+  Definition t := uvar.
+  Definition eq := @eq uvar.
+  Definition lt := @lt.
+
+  Theorem eq_refl : forall x, eq x x.
+  Proof. reflexivity. Qed.
+
+  Theorem eq_sym : forall a b, eq a b -> eq b a.
+  Proof. intros; symmetry; auto. Qed.
+
+  Theorem eq_trans : forall a b c, eq a b -> eq b c -> eq a c.
+  Proof. intros; etransitivity; eauto. Qed.
+
+  Theorem lt_trans : forall a b c, lt a b -> lt b c -> lt a c.
+  Proof. eapply Lt.lt_trans. Qed.
+
+  Theorem lt_not_eq : forall a b, lt a b -> ~(eq a b).
+  Proof. eapply NPeano.Nat.lt_neq. Qed.
+
+  Definition compare (x y : t) : OrderedType.Compare lt eq x y :=
+    match Compare_dec.nat_compare x y as r return
+      Compare_dec.nat_compare x y = r -> OrderedType.Compare lt eq x y
+      with
+      | Lt => fun pf => OrderedType.LT (lt:=lt) (Compare_dec.nat_compare_Lt_lt _ _ pf)
+      | Eq => fun pf => OrderedType.EQ (lt:=lt) (Compare_dec.nat_compare_eq _ _ pf)
+      | Gt => fun pf => OrderedType.GT (lt:=lt) (Compare_dec.nat_compare_Gt_gt _ _ pf)
+    end (refl_equal _).
+
+  Definition eq_dec (x y : nat) : {x = y} + {x <> y} :=
+    match EqNat.beq_nat x y as r return
+      EqNat.beq_nat x y = r -> {x = y} + {x <> y} with
+      | true => fun pf => left (EqNat.beq_nat_true _ _ pf)
+      | false => fun pf => right (EqNat.beq_nat_false _ _ pf)
+    end (refl_equal _).
+End UVar_ord.
+
+Module MAP <: WS with Definition E.t := uvar
+                 with Definition E.eq := @eq uvar.
+  Module E := UVar_ord.
+
+  Definition to_key : uvar -> positive :=
+    Pos.of_succ_nat.
+
+  Definition from_key : positive -> uvar :=
+    fun p => pred (Pos.to_nat p).
+
+  Definition key := uvar.
+  Hint Transparent key.
+
+  Definition t : Type -> Type := PositiveMap.t.
+  (** the abstract type of maps *)
+
+  Section Types.
+
+    Variable elt:Type.
+
+    Definition empty : t elt :=
+      Eval red in PositiveMap.empty _.
+    (** The empty map. *)
+
+    Definition is_empty : t elt -> bool :=
+      Eval red in @PositiveMap.is_empty _.
+    (** Test whether a map is empty or not. *)
+
+    Definition add (k : key) : elt -> t elt -> t elt :=
+      Eval red in PositiveMap.add (to_key k).
+    (** [add x y m] returns a map containing the same bindings as [m],
+	plus a binding of [x] to [y]. If [x] was already bound in [m],
+	its previous binding disappears. *)
+
+    Definition find (k : key) : t elt -> option elt :=
+      Eval red in PositiveMap.find (to_key k).
+    (** [find x m] returns the current binding of [x] in [m],
+	or [None] if no such binding exists. *)
+
+    Definition remove (k : key) : t elt -> t elt :=
+      Eval red in PositiveMap.remove (to_key k).
+    (** [remove x m] returns a map containing the same bindings as [m],
+	except for [x] which is unbound in the returned map. *)
+
+    Definition mem (k : key) : t elt -> bool :=
+      Eval red in PositiveMap.mem (to_key k).
+    (** [mem x m] returns [true] if [m] contains a binding for [x],
+	and [false] otherwise. *)
+
+    Variable elt' elt'' : Type.
+
+    Definition map : (elt -> elt') -> t elt -> t elt' :=
+      Eval red in @PositiveMap.map _ _.
+    (** [map f m] returns a map with same domain as [m], where the associated
+	value a of all bindings of [m] has been replaced by the result of the
+	application of [f] to [a]. Since Coq is purely functional, the order
+        in which the bindings are passed to [f] is irrelevant. *)
+
+    Definition mapi (f : key -> elt -> elt') : t elt -> t elt' :=
+      Eval red in @PositiveMap.mapi _ _ (fun k v => f (from_key k) v).
+    (** Same as [map], but the function receives as arguments both the
+	key and the associated value for each binding of the map. *)
+
+    Definition map2 :
+     (option elt -> option elt' -> option elt'') -> t elt -> t elt' ->  t elt'' :=
+      Eval red in @PositiveMap.map2 _ _ _.
+    (** [map2 f m m'] creates a new map whose bindings belong to the ones
+        of either [m] or [m']. The presence and value for a key [k] is
+        determined by [f e e'] where [e] and [e'] are the (optional) bindings
+        of [k] in [m] and [m']. *)
+
+    Definition elements (m : t elt) : list (key*elt) :=
+      Eval red in List.map (fun kv => let '(k,v) := kv in
+                                      (from_key k, v)) (PositiveMap.elements m).
+    (** [elements m] returns an assoc list corresponding to the bindings
+        of [m], in any order. *)
+
+    Definition cardinal : t elt -> nat :=
+      Eval red in @PositiveMap.cardinal _.
+    (** [cardinal m] returns the number of bindings in [m]. *)
+
+    Definition fold (A: Type) (f : key -> elt -> A -> A) : t elt -> A -> A :=
+      Eval red in @PositiveMap.fold _ A (fun k => f (from_key k)).
+      
+    (** [fold f m a] computes [(f kN dN ... (f k1 d1 a)...)],
+	where [k1] ... [kN] are the keys of all bindings in [m]
+	(in any order), and [d1] ... [dN] are the associated data. *)
+
+    Definition equal : (elt -> elt -> bool) -> t elt -> t elt -> bool :=
+      Eval red in @PositiveMap.equal _.
+    (** [equal cmp m1 m2] tests whether the maps [m1] and [m2] are equal,
+      that is, contain equal keys and associate them with equal data.
+      [cmp] is the equality predicate used to compare the data associated
+      with the keys. *)
+
+    Section Spec.
+
+      Variable m m' m'' : t elt.
+      Variable x y z : key.
+      Variable e e' : elt.
+
+      Definition MapsTo (k : key) : elt -> t elt -> Prop :=
+        PositiveMap.MapsTo (to_key k).
+
+      Definition In (k:key)(m: t elt) : Prop := exists e:elt, MapsTo k e m.
+
+      Definition Empty m := forall (a : key)(e:elt) , ~ MapsTo a e m.
+
+      Definition eq_key (p p':key*elt) := E.eq (fst p) (fst p').
+
+      Definition eq_key_elt (p p':key*elt) :=
+          E.eq (fst p) (fst p') /\ (snd p) = (snd p').
+
+    (** Specification of [MapsTo] *)
+      Theorem MapsTo_1 : E.eq x y -> MapsTo x e m -> MapsTo y e m.
+      Admitted.
+
+    (** Specification of [mem] *)
+      Theorem mem_1 : In x m -> mem x m = true.
+      Admitted.
+      Theorem mem_2 : mem x m = true -> In x m.
+      Admitted.
+
+    (** Specification of [empty] *)
+      Theorem empty_1 : Empty empty.
+      Admitted.
+
+    (** Specification of [is_empty] *)
+      Theorem is_empty_1 : Empty m -> is_empty m = true.
+      Admitted.
+      Theorem is_empty_2 : is_empty m = true -> Empty m.
+      Admitted.
+
+    (** Specification of [add] *)
+      Theorem add_1 : E.eq x y -> MapsTo y e (add x e m).
+      Admitted.
+      Theorem add_2 : ~ E.eq x y -> MapsTo y e m -> MapsTo y e (add x e' m).
+      Admitted.
+      Theorem add_3 : ~ E.eq x y -> MapsTo y e (add x e' m) -> MapsTo y e m.
+      Admitted.
+
+    (** Specification of [remove] *)
+      Theorem remove_1 : E.eq x y -> ~ In y (remove x m).
+      Admitted.
+      Theorem remove_2 : ~ E.eq x y -> MapsTo y e m -> MapsTo y e (remove x m).
+      Admitted.
+      Theorem remove_3 : MapsTo y e (remove x m) -> MapsTo y e m.
+      Admitted.
+
+    (** Specification of [find] *)
+      Theorem find_1 : MapsTo x e m -> find x m = Some e.
+      Admitted.
+      Theorem find_2 : find x m = Some e -> MapsTo x e m.
+      Admitted.
+
+    (** Specification of [elements] *)
+      Theorem elements_1 :
+        MapsTo x e m -> InA eq_key_elt (x,e) (elements m).
+      Admitted.
+      Theorem elements_2 :
+        InA eq_key_elt (x,e) (elements m) -> MapsTo x e m.
+      Admitted.
+      (** When compared with ordered maps, here comes the only
+         property that is really weaker: *)
+      Theorem elements_3w : NoDupA eq_key (elements m).
+      Admitted.
+
+    (** Specification of [cardinal] *)
+      Theorem cardinal_1 : cardinal m = length (elements m).
+      Admitted.
+
+    (** Specification of [fold] *)
+      Theorem fold_1 :
+	forall (A : Type) (i : A) (f : key -> elt -> A -> A),
+        fold f m i = fold_left (fun a p => f (fst p) (snd p) a) (elements m) i.
+      Admitted.
+
+    (** Equality of maps *)
+
+    (** Caveat: there are at least three distinct equality predicates on maps.
+      - The simpliest (and maybe most natural) way is to consider keys up to
+        their equivalence [E.eq], but elements up to Leibniz equality, in
+        the spirit of [eq_key_elt] above. This leads to predicate [Equal].
+      - Unfortunately, this [Equal] predicate can't be used to describe
+        the [equal] function, since this function (for compatibility with
+        ocaml) expects a boolean comparison [cmp] that may identify more
+        elements than Leibniz. So logical specification of [equal] is done
+        via another predicate [Equivb]
+      - This predicate [Equivb] is quite ad-hoc with its boolean [cmp],
+        it can be generalized in a [Equiv] expecting a more general
+        (possibly non-decidable) equality predicate on elements *)
+
+     Definition Equal m m' := forall y, find y m = find y m'.
+     Definition Equiv (eq_elt:elt->elt->Prop) m m' :=
+         (forall k, In k m <-> In k m') /\
+         (forall k e e', MapsTo k e m -> MapsTo k e' m' -> eq_elt e e').
+     Definition Equivb (cmp: elt->elt->bool) := Equiv (Cmp cmp).
+
+     (** Specification of [equal] *)
+
+     Variable cmp : elt -> elt -> bool.
+
+     Theorem equal_1 : Equivb cmp m m' -> equal cmp m m' = true.
+     Admitted.
+     Theorem equal_2 : equal cmp m m' = true -> Equivb cmp m m'.
+     Admitted.
+
+    End Spec.
+   End Types.
+
+    (** Specification of [map] *)
+      Parameter map_1 : forall (elt elt':Type)(m: t elt)(x:key)(e:elt)(f:elt->elt'),
+        MapsTo x e m -> MapsTo x (f e) (map f m).
+      Parameter map_2 : forall (elt elt':Type)(m: t elt)(x:key)(f:elt->elt'),
+        In x (map f m) -> In x m.
+
+    (** Specification of [mapi] *)
+      Parameter mapi_1 : forall (elt elt':Type)(m: t elt)(x:key)(e:elt)
+        (f:key->elt->elt'), MapsTo x e m ->
+        exists y, E.eq y x /\ MapsTo x (f y e) (mapi f m).
+      Parameter mapi_2 : forall (elt elt':Type)(m: t elt)(x:key)
+        (f:key->elt->elt'), In x (mapi f m) -> In x m.
+
+    (** Specification of [map2] *)
+      Parameter map2_1 : forall (elt elt' elt'':Type)(m: t elt)(m': t elt')
+	(x:key)(f:option elt->option elt'->option elt''),
+	In x m \/ In x m' ->
+        find x (map2 f m m') = f (find x m) (find x m').
+
+     Parameter map2_2 : forall (elt elt' elt'':Type)(m: t elt)(m': t elt')
+	(x:key)(f:option elt->option elt'->option elt''),
+        In x (map2 f m m') -> In x m \/ In x m'.
+End MAP.
+
+Require Coq.FSets.FMapAVL.
+
+Module MAP2 := FMapAVL.Make UVar_ord.
